@prefix owl:    <http://www.w3.org/2002/07/owl#> .
@prefix soma:   <http://www.ease-crc.org/ont/SOMA.owl#> .
@prefix dul:    <http://www.ontologydesignpatterns.org/ont/dul/DUL.owl#> .
@prefix geo:    <http://www.opengis.net/ont/geosparql#> .
@prefix xsd:    <http://www.w3.org/2001/XMLSchema#> .
@prefix rdf:    <http://www.w3.org/1999/02/22-rdf-syntax-ns#> .
@prefix rdfs:   <http://www.w3.org/2000/01/rdf-schema#> .
@prefix :       <http://find-a-name.org/> .

###################################
# CLASSES
###################################

:Instruction a owl:Class ;
    rdfs:label "Instruction"@en ;
    rdfs:comment "An instruction is a command or directive given to a system or user."@en .

:Workflow a owl:Class ;
    rdfs:subClassOf dul:Workflow ;
    rdfs:label "Workflow"@en ;
    rdfs:comment "A workflow is a sequence of tasks or processes that are carried out to fulfil the instruction."@en .

:Task a owl:Class ;
    rdfs:subClassOf dul:Task ;
    rdfs:label "Task"@en ;
    rdfs:comment "A task is a specific piece of work or activity that is part of a workflow."@en .

:Action a owl:Class ;
    rdfs:subClassOf dul:Action ;
    rdfs:label "Action"@en ;
    rdfs:comment "An action is a specific operation or function that can be performed as part of a task."@en .

:Agent a owl:Class ;
    rdfs:subClassOf dul:Agent ;
    rdfs:label "Agent"@en ;
    rdfs:comment "An agent is an entity that can perform actions or tasks."@en .

:Component a owl:Class ;
    rdfs:subClassOf dul:Entity ;
    rdfs:label "Component"@en ;
    rdfs:comment "A component is a part of a system that can be used to perform tasks or actions."@en .

:Appliance a dul:Component ;
    rdfs:label "Appliance"@en ;
    rdfs:comment "An appliance is a device or machine that performs a specific function."@en .

:Furniture a dul:Component ;
    rdfs:label "Furniture"@en ;
    rdfs:comment "Furniture refers to movable objects intended to support various human activities."@en .

:Object a dul:Component ;
    rdfs:label "Object"@en ;
    rdfs:comment "An object is a material thing that can be perceived by the senses."@en .

:Location a owl:Class ;
    rdfs:subClassOf soma:Location ;
    rdfs:label "Location"@en ;
    rdfs:comment "A location is a specific place or position where an action or task can take place."@en .

:Environment a owl:Class ;
    rdfs:subClassOf dul:Entity ;
    rdfs:label "Environment"@en ;
    rdfs:comment "An environment is a surrounding area or context in which an action or task occurs."@en .

:StateType a owl:Class ;
    rdfs:subClassOf soma:StateType ;
    rdfs:label "State Type"@en ;
    rdfs:comment "A state type is a specific condition of the environment."@en .

:InitialState a :StateType ;
    rdfs:label "Initial State"@en ;
    rdfs:comment "The initial state of the environment before any actions are performed."@en .

:CurrentState a :StateType ;
    rdfs:label "Current State"@en ;
    rdfs:comment "The current state of the environment during the execution of actions."@en .

:FinalState a :StateType ;
    rdfs:label "Final State"@en ;
    rdfs:comment "The final state of the environment after all actions have been performed."@en .

###################################
# OBJECT PROPERTIES
###################################

:hasWorkflow a owl:ObjectProperty ;
    rdfs:domain :Instruction ;
    rdfs:range :Workflow ;
    rdfs:label "has workflow"@en ;
    rdfs:comment "An instruction has a workflow that needs to be executed."@en .

:hasTask a owl:ObjectProperty ;
    rdfs:subPropertyOf dul:hasTask ;
    rdfs:domain :Workflow ;
    rdfs:range :Task ;
    rdfs:label "has task"@en ;
    rdfs:comment "A workflow consists of one or more tasks."@en .

:precedes a owl:ObjectProperty ;
    rdfs:subPropertyOf dul:precedes ;
    rdfs:domain :Task ;
    rdfs:range :Task ;
    rdfs:label "precedes"@en ;
    rdfs:comment "A task can precede another task in a workflow."@en .

:follows a owl:ObjectProperty ;
    rdfs:subPropertyOf dul:follows ;
    rdfs:domain :Task ;
    rdfs:range :Task ;
    rdfs:label "follows"@en ;
    rdfs:comment "A task can follow another task in a workflow."@en .

:isExecutedIn a owl:ObjectProperty ;
    rdfs:subPropertyOf dul:isExecutedIn ;
    rdfs:domain :Task ;
    rdfs:range :Action ;
    rdfs:label "is executed in"@en ;
    rdfs:comment "A task is executed in the context of an action."@en .

:isPerformedBy a owl:ObjectProperty ;
    rdfs:subPropertyOf soma:isPerformedBy ;
    rdfs:domain :Action ;
    rdfs:range :Agent ;
    rdfs:label "is performed by"@en ;
    rdfs:comment "An action is performed by an agent."@en .

:hasComponent a owl:ObjectProperty ;
    rdfs:subPropertyOf dul:hasComponent ;
    rdfs:domain :Action ;
    rdfs:range :Component ;
    rdfs:label "has component"@en ;
    rdfs:comment "An action can have one or more components."@en .

:hasLocation a owl:ObjectProperty ;
    rdfs:subPropertyOf dul:hasLocation ;
    rdfs:domain :Component ;
    rdfs:range :Location ;
    rdfs:label "has location"@en ;
    rdfs:comment "A component can have a specific location."@en .

:contains a owl:ObjectProperty ;
    rdfs:subPropertyOf geo:sfContains ;
    rdfs:domain :Location ;
    rdfs:range :Component ;
    rdfs:label "contains"@en ;
    rdfs:comment "A location can contain other locations."@en .

:within a owl:ObjectProperty ;
    rdfs:subPropertyOf geo:sfWithin ;
    rdfs:domain :Component ;
    rdfs:range :Location ;
    rdfs:label "within"@en ;
    rdfs:comment "A component can be within a specific location."@en .

:overlaps a owl:ObjectProperty ;
    rdfs:subPropertyOf geo:sfOverlaps ;
    rdfs:domain :Location ;
    rdfs:range :Location ;
    rdfs:label "overlaps"@en ;
    rdfs:comment "Two locations can overlap each other."@en .

:hasComponentType a owl:ObjectProperty ;
    rdfs:subPropertyOf dul:hasComponent ;
    rdfs:domain :Environment ;
    rdfs:range :Component ;
    rdfs:label "has component type"@en ;
    rdfs:comment "An Environment can have one or more components."@en .

:hasStateType a owl:ObjectProperty ;
    rdfs:subPropertyOf soma:hasStateType ;
    rdfs:domain :Environment ;
    rdfs:range :StateType ;
    rdfs:label "has state type"@en ;
    rdfs:comment "An Environment can have one or more state types."@en .

###################################
# DATA PROPERTIES
###################################

:hasNaturalLanguage a owl:DatatypeProperty ;
    rdfs:domain :Instruction ;
    rdfs:range xsd:string ;
    rdfs:label "has natural language"@en ;
    rdfs:comment "The instruction is expressed in a natural language."@en .

:asWKT a owl:DatatypeProperty ;
    rdfs:subPropertyOf soma:asWKT ;
    rdfs:domain :Location ;
    rdfs:range xsd:string ;
    rdfs:label "as WKT"@en ;
    rdfs:comment "The location is represented in Well-Known Text (WKT) format."@en .
