@prefix owl:    <http://www.w3.org/2002/07/owl#> .
@prefix soma:   <http://www.ease-crc.org/ont/SOMA.owl#> .
@prefix dul:    <http://www.ontologydesignpatterns.org/ont/dul/DUL.owl#> .
@prefix geo:    <http://www.opengis.net/ont/geosparql#> .
@prefix xsd:    <http://www.w3.org/2001/XMLSchema#> .
@prefix rdf:    <http://www.w3.org/1999/02/22-rdf-syntax-ns#> .
@prefix rdfs:   <http://www.w3.org/2000/01/rdf-schema#> .
@prefix :       <http://find-a-name.org/> .

###################################
# CLASSES
###################################

:Instruction a owl:Class, dul:Entity ;
    rdfs:label "Instruction"@en ;
    rdfs:comment "An instruction is a command or directive given to a system or user."@en .

:Workflow a owl:Class, dul:Entity ;
    rdfs:subClassOf dul:Workflow ;
    rdfs:label "Workflow"@en ;
    rdfs:comment "A workflow is a sequence of tasks or processes that are carried out to fulfil the instruction."@en .

:Component a owl:Class, dul:Entity ;
    rdfs:subClassOf dul:Entity ;
    rdfs:label "Component"@en ;
    rdfs:comment "A component is a part of a system that can be used to perform tasks or actions."@en .

:Affordance a owl:Class, dul:Entity ;
    rdfs:label "Affordance"@en ;
    rdfs:comment "An affordance is a property of an object that indicates how it can be used."@en .

:Appliance a owl:Class, dul:Entity ;
    rdfs:label "Appliance"@en ;
    rdfs:comment "An appliance is a device or machine that performs a specific function."@en .

:Furniture a owl:Class, dul:Entity ;
    rdfs:label "Furniture"@en ;
    rdfs:comment "Furniture refers to movable objects intended to support various human activities."@en .

:Object a owl:Class, dul:Entity ;
    rdfs:label "Object"@en ;
    rdfs:comment "An object is a material thing that can be perceived by the senses."@en .

:Environment a owl:Class, dul:Entity ;
    rdfs:subClassOf dul:Entity ;
    rdfs:label "Environment"@en ;
    rdfs:comment "An environment is a surrounding area or context in which an action or task occurs."@en .

:InitialState a owl:Class, dul:Entity, soma:StateType ;
    rdfs:label "Initial State"@en ;
    rdfs:comment "The initial state of the environment before any actions are performed."@en .

:CurrentState a owl:Class, dul:Entity, soma:StateType ;
    rdfs:label "Current State"@en ;
    rdfs:comment "The current state of the environment during the execution of actions."@en .

:FinalState a owl:Class, dul:Entity, soma:StateType ;
    rdfs:label "Final State"@en ;
    rdfs:comment "The final state of the environment after all actions have been performed."@en .

###################################
# OBJECT PROPERTIES
###################################

:hasWorkflow a owl:ObjectProperty ;
    rdfs:domain :Instruction ;
    rdfs:range :Workflow ;
    rdfs:label "has workflow"@en ;
    rdfs:comment "An instruction has a workflow that needs to be executed."@en .

:hasTask a owl:ObjectProperty ;
    rdfs:subPropertyOf dul:hasTask ;
    rdfs:domain :Workflow ;
    rdfs:range dul:Task ;
    rdfs:label "has task"@en ;
    rdfs:comment "A workflow consists of one or more tasks."@en .

:actsOn a owl:ObjectProperty ;
    rdfs:domain :Action ;
    rdfs:range :Component ;
    rdfs:label "acts on"@en ;
    rdfs:comment "An action is acted on one or more components."@en .

:hasAffordance a owl:ObjectProperty ;
    rdfs:domain :Component ;
    rdfs:range :Affordance ;
    rdfs:label "has affordance"@en ;
    rdfs:comment "A component has one or more affordances that indicate how it can be used."@en .

:isAffordedBy a owl:ObjectProperty ;
    rdfs:domain :Action ;
    rdfs:range :Affordance ;
    rdfs:label "is afforded by"@en ;
    rdfs:comment "An action is afforded by one affordance."@en .

###################################
# DATA PROPERTIES
###################################

:hasNaturalLanguage a owl:DatatypeProperty ;
    rdfs:domain :Instruction ;
    rdfs:range xsd:string ;
    rdfs:label "has natural language"@en ;
    rdfs:comment "The instruction is expressed in a natural language."@en .